LTT_PLTT.v
@@ -1,0 +1,636 @@
+Require Import Common.
+Require Import Traces.
+Require Import Machine.
+Require Import LTT.
+Require Import PLTT.
+
+Module LTT_TO_PLTT.
+
+Include AbstractMachine.
+
+Inductive match_states (split : list Component.id)
+  : LTT.state -> PLTT.partial_state -> Prop :=
+| program_control:
+    forall C s ps mem pmem regs pc,
+      PLTT.is_program_component C split ->
+      ps = PLTT.to_partial_stack s split ->
+      PLTT.maps_match_on split mem pmem ->
+      match_states split
+                   (C, s, mem, regs, pc)
+                   (PLTT.PC (C, ps, pmem, regs, pc))
+
+| context_control:
+    forall C s ps mem pmem regs pc,
+      PLTT.is_context_component C split ->
+      ps = PLTT.to_partial_stack s split ->
+      PLTT.maps_match_on split mem pmem ->
+      match_states split
+                   (C, s, mem, regs, pc)
+                   (PLTT.CC (C, ps, pmem)).
+
+Definition memory_wf (Is : list Component.interface) (mem : Memory.data) :=
+  forall CI C,
+    In CI Is -> Component.name CI = C ->
+    exists Cmem, M.MapsTo C Cmem mem.
+
+Theorem option_simulation:
+  forall split s C d mem regs pc s' ps Is E t,
+    let G := LTT.mkGlobalEnv Is E in
+    s = (C,d,mem,regs,pc) ->
+
+    (* Global environment well-formedness *)
+    (* - entrypoints exist for each declared component *)
+    LTT.global_env_wf G ->
+
+    (* Memory well-formedness *)
+    (* - each declared component has its own memory *)
+    memory_wf (LTT.get_interfaces G) mem ->
+
+    (* Simulation premises *)
+    match_states split s ps ->
+    LTT.step G s t s' ->
+
+    (* Simulation argument *)
+    (t = E0 /\ match_states split s' ps)
+    \/
+    (forall E',
+        (* Entrypoints preservation *)
+        PLTT.maps_match_on split E E' ->
+        (* Global environment well-formedness *)
+        let G' := PLTT.mkGlobalEnv Is E' split in
+        PLTT.global_env_wf G' ->
+        (* Simulation step *)
+        exists ps',
+          PLTT.step G' ps t ps' /\ match_states split s' ps').
+Proof.
+  intros split s C d mem regs pc s' ps Is E t.
+  intros G Hstate HGwf HmemWF Hstates_match Hstep.
+
+  inversion Hstates_match as [ C0 ? ? ? ? ? ? Hcontrol Hpstack Hmem |
+                               C0 ? ? ? ? ? ? Hcontrol Hpstack Hmem ];
+    inversion Hstep;
+    rewrite Hpstack;
+    match goal with
+    | Hstate'  : (C0, _, _, _, _) = s,
+      Hstate'' : (_, _, _, _, _) = s |- _ =>
+      rewrite <- Hstate'' in Hstate'; inversion Hstate'; subst
+    end;
+
+    (* prove context epsilon steps by staying still *)
+    try (left; split; 
+         [ reflexivity
+         | apply context_control;
+           try assumption;
+           try reflexivity;
+           try apply Hmem]).
+
+  (* program epsilon steps *)
+  - right.
+    intros E' HE'WF G' HG'WF.
+    eexists. split.
+    (* step *)
+    + destruct (PLTT.split_wellformed G' HG'WF C1 Hcontrol)
+        as [C1I [C1_in_Is C1I_name]].
+      destruct (HmemWF C1I C1 C1_in_Is C1I_name) as [C1mem HC1mem].
+      eapply PLTT.Program_Epsilon.
+      * apply HC1mem.
+      * apply HC1mem.
+      * simpl. unfold PLTT.maps_match_on.
+        intros. split; intro; apply HE'WF; assumption.
+      * simpl. rewrite H2 in H.
+        inversion H.
+        rewrite H3 in Hstep.
+        rewrite H4 in Hstep.
+        rewrite H5 in Hstep.
+        rewrite H6 in Hstep.
+        rewrite H7 in Hstep.
+        eapply Hstep.
+      * apply Hmem. assumption.
+        rewrite H2 in H.
+        inversion H.
+        rewrite <- H3. assumption.
+      * eassumption.
+    (* states match *)
+    + simpl. rewrite H2 in H.
+      inversion H.
+      rewrite <- H7.
+      apply program_control.
+      rewrite <- H3. assumption.
+      reflexivity.
+      simpl. unfold PLTT.maps_match_on.
+      intros. split; intro; assumption.
+
+  - right.
+    intros E' HE'WF G' HG'WF.
+    eexists. split.
+    (* step *)
+    + destruct (PLTT.split_wellformed G' HG'WF C1 Hcontrol)
+        as [C1I [C1_in_Is C1I_name]].
+      destruct (HmemWF C1I C1 C1_in_Is C1I_name) as [C1mem HC1mem].
+      eapply PLTT.Program_Epsilon.
+      * apply HC1mem.
+      * apply HC1mem.
+      * simpl. unfold PLTT.maps_match_on.
+        intros. split; intro; apply HE'WF; assumption.
+      * simpl. rewrite H3 in H.
+        inversion H.
+        rewrite H2 in Hstep.
+        rewrite H4 in Hstep.
+        rewrite H5 in Hstep.
+        rewrite H6 in Hstep.
+        rewrite H7 in Hstep.
+        eapply Hstep.
+      * apply Hmem. assumption.
+        rewrite H3 in H.
+        inversion H.
+        rewrite <- H2. assumption.
+      * eassumption.
+    (* states match *)
+    + simpl. rewrite H3 in H.
+      inversion H.
+      rewrite <- H7.
+      apply program_control.
+      rewrite <- H2. assumption.
+      reflexivity.
+      simpl. unfold PLTT.maps_match_on.
+      intros. split; intro; assumption.
+
+  - right.
+    intros E' HE'WF G' HG'WF.
+    eexists. split.
+    (* step *)
+    + destruct (PLTT.split_wellformed G' HG'WF C1 Hcontrol)
+        as [C1I [C1_in_Is C1I_name]].
+      destruct (HmemWF C1I C1 C1_in_Is C1I_name) as [C1mem HC1mem].
+      eapply PLTT.Program_Epsilon.
+      * apply HC1mem.
+      * apply HC1mem.
+      * simpl. unfold PLTT.maps_match_on.
+        intros. split; intro; apply HE'WF; assumption.
+      * simpl. rewrite H3 in H.
+        inversion H.
+        rewrite H2 in Hstep.
+        rewrite H4 in Hstep.
+        rewrite H5 in Hstep.
+        rewrite H6 in Hstep.
+        rewrite H7 in Hstep.
+        eapply Hstep.
+      * apply Hmem. assumption.
+        rewrite H3 in H.
+        inversion H.
+        rewrite <- H2. assumption.
+      * eassumption.
+    (* states match *)
+    + simpl. rewrite H3 in H.
+      inversion H.
+      rewrite <- H7.
+      apply program_control.
+      rewrite <- H2. assumption.
+      reflexivity.
+      simpl. unfold PLTT.maps_match_on.
+      intros. split; intro; assumption.
+
+  - right.
+    intros E' HE'WF G' HG'WF.
+    eexists. split.
+    (* step *)
+    + destruct (PLTT.split_wellformed G' HG'WF C1 Hcontrol)
+        as [C1I [C1_in_Is C1I_name]].
+      destruct (HmemWF C1I C1 C1_in_Is C1I_name) as [C1mem HC1mem].
+      eapply PLTT.Program_Epsilon.
+      * apply HC1mem.
+      * apply HC1mem.
+      * simpl. unfold PLTT.maps_match_on.
+        intros. split; intro; apply HE'WF; assumption.
+      * simpl. rewrite H5 in H.
+        inversion H.
+        rewrite H2 in Hstep.
+        rewrite H3 in Hstep.
+        rewrite H4 in Hstep.
+        rewrite H6 in Hstep.
+        rewrite H7 in Hstep.
+        eapply Hstep.
+      * apply Hmem. assumption.
+        rewrite H5 in H.
+        inversion H.
+        rewrite <- H2. assumption.
+      * eassumption.
+    (* states match *)
+    + simpl. rewrite H5 in H.
+      inversion H.
+      rewrite <- H7.
+      apply program_control.
+      rewrite <- H2. assumption.
+      reflexivity.
+      simpl. unfold PLTT.maps_match_on.
+      intros. split; intro; assumption.
+
+  - right.
+    intros E' HE'WF G' HG'WF.
+    eexists. split.
+    (* step *)
+    + destruct (PLTT.split_wellformed G' HG'WF C1 Hcontrol)
+        as [C1I [C1_in_Is C1I_name]].
+      destruct (HmemWF C1I C1 C1_in_Is C1I_name) as [C1mem HC1mem].
+      eapply PLTT.Program_Epsilon.
+      * apply HC1mem.
+      * apply HC1mem.
+      * simpl. unfold PLTT.maps_match_on.
+        intros. split; intro; apply HE'WF; assumption.
+      * simpl. rewrite H5 in H.
+        inversion H.
+        rewrite H2 in Hstep.
+        rewrite H4 in Hstep.
+        rewrite H6 in Hstep.
+        rewrite H7 in Hstep.
+        rewrite H8 in Hstep.
+        eapply Hstep.
+      * apply Hmem. assumption.
+        rewrite H5 in H.
+        inversion H.
+        rewrite <- H2. assumption.
+      * eassumption.
+    (* states match *)
+    + simpl. rewrite H5 in H.
+      inversion H.
+      rewrite <- H7.
+      apply program_control.
+      rewrite <- H2. assumption.
+      reflexivity.
+      simpl. unfold PLTT.maps_match_on.
+      intros. split; intro; assumption.
+
+  (* store *)
+  - right. intros E' HE'WF G' HG'WF.
+    exists (PLTT.PC (C1, PLTT.to_partial_stack d0 split,
+                     Memory.set pmem C1
+                                (Register.get r1 regs1)
+                                (Register.get r2 regs1),
+                     regs1, pc1+1)).
+    split.
+    (* step *)
+    + destruct (PLTT.split_wellformed G' HG'WF C1 Hcontrol)
+        as [C1I [C1_in_Is C1I_name]].
+      destruct (HmemWF C1I C1 C1_in_Is C1I_name)
+        as [C1mem HC1mem].
+      eapply PLTT.Program_Epsilon with
+        (s:=d) (cmem:=C1mem)
+        (cmem':=Memory.local_update
+                  (Register.get r1 regs1)
+                  (Register.get r2 regs1) C1mem)
+        (wmem':=M.add C1
+                      (Memory.local_update
+                         (Register.get r1 regs1)
+                         (Register.get r2 regs1) C1mem)
+                      mem1).
+      * apply HC1mem.
+      * apply M.add_1. reflexivity.
+      * unfold G'. simpl.
+        unfold PLTT.maps_match_on.
+        intros. split; intro; apply HE'WF; assumption.
+      * simpl. 
+        unfold G in Hstep.
+        rewrite H5 in H. inversion H.
+        rewrite H2,H3,H4,H6,H7 in Hstep.
+        unfold Memory.set in Hstep.
+        rewrite H2 in HC1mem.
+        rewrite (M.find_1 HC1mem) in Hstep.
+        apply Hstep.
+      * apply Hmem. assumption.
+        rewrite H5 in H. inversion H.
+        rewrite <- H2. assumption.
+      * unfold Memory.set.
+        rewrite H5 in H. inversion H.
+        rewrite <- H4 in HC1mem.
+        apply Hmem in HC1mem.
+        rewrite H2 in HC1mem.
+        rewrite (M.find_1 HC1mem).
+        apply M.add_1.
+        ** reflexivity.
+        ** assumption.
+    (* states match *)
+    + apply program_control.
+      * assumption.
+      * reflexivity.
+      * apply PLTT.update_related_memories with
+          (C:=C1) (mem1:=mem1) (mem2:=pmem)
+          (addr:=Register.get r1 regs1)
+          (val:=Register.get r2 regs1);
+          try assumption;
+          reflexivity.
+
+  - right.
+    intros E' HE'WF G' HG'WF.
+    eexists. split.
+    (* step *)
+    + destruct (PLTT.split_wellformed G' HG'WF C1 Hcontrol)
+        as [C1I [C1_in_Is C1I_name]].
+      destruct (HmemWF C1I C1 C1_in_Is C1I_name)
+        as [C1mem HC1mem].
+      eapply PLTT.Program_Epsilon.
+      * apply HC1mem.
+      * apply HC1mem.
+      * simpl. unfold PLTT.maps_match_on.
+        intros. split; intro; apply HE'WF; assumption.
+      * simpl. rewrite H4 in H.
+        inversion H.
+        rewrite H2 in Hstep.
+        rewrite H3 in Hstep.
+        rewrite H5 in Hstep.
+        rewrite H6 in Hstep.
+        rewrite H7 in Hstep.
+        eapply Hstep.
+      * apply Hmem. assumption.
+        rewrite H4 in H.
+        inversion H.
+        rewrite <- H2. assumption.
+      * eassumption.
+    (* states match *)
+    + simpl. rewrite H4 in H.
+      inversion H.
+      rewrite <- H7.
+      apply program_control.
+      rewrite <- H2. assumption.
+      reflexivity.
+      simpl. unfold PLTT.maps_match_on.
+      intros. split; intro; assumption.
+
+  - right.
+    intros E' HE'WF G' HG'WF.
+    eexists. split.
+    (* step *)
+    + destruct (PLTT.split_wellformed G' HG'WF C1 Hcontrol)
+        as [C1I [C1_in_Is C1I_name]].
+      destruct (HmemWF C1I C1 C1_in_Is C1I_name)
+        as [C1mem HC1mem].
+      eapply PLTT.Program_Epsilon.
+      * apply HC1mem.
+      * apply HC1mem.
+      * simpl. unfold PLTT.maps_match_on.
+        intros. split; intro; apply HE'WF; assumption.
+      * simpl. rewrite H3 in H.
+        inversion H.
+        rewrite H2 in Hstep.
+        rewrite H4 in Hstep.
+        rewrite H5 in Hstep.
+        rewrite H6 in Hstep.
+        eapply Hstep.
+      * apply Hmem. assumption.
+        rewrite H3 in H.
+        inversion H.
+        rewrite <- H2. assumption.
+      * eassumption.
+    (* states match *)
+    + simpl. rewrite H3 in H.
+      inversion H.
+      (* NOTE here we don't rewrite *)
+      apply program_control.
+      rewrite <- H2. assumption.
+      reflexivity.
+      simpl. unfold PLTT.maps_match_on.
+      intros. split; intro; assumption.
+
+  - right.
+    intros E' HE'WF G' HG'WF.
+    eexists. split.
+    (* step *)
+    + destruct (PLTT.split_wellformed G' HG'WF C1 Hcontrol)
+        as [C1I [C1_in_Is C1I_name]].
+      destruct (HmemWF C1I C1 C1_in_Is C1I_name)
+        as [C1mem HC1mem].
+      eapply PLTT.Program_Epsilon.
+      * apply HC1mem.
+      * apply HC1mem.
+      * simpl. unfold PLTT.maps_match_on.
+        intros. split; intro; apply HE'WF; assumption.
+      * simpl. rewrite H3 in H.
+        inversion H.
+        rewrite H4 in Hstep.
+        rewrite H5 in Hstep.
+        rewrite H6 in Hstep.
+        rewrite H7 in Hstep.
+        rewrite H8 in Hstep.
+        eapply Hstep.
+      * apply Hmem. assumption.
+        rewrite H3 in H.
+        inversion H.
+        rewrite <- H4. assumption.
+      * eassumption.
+    (* states match *)
+    + simpl. rewrite H3 in H.
+      inversion H.
+      rewrite <- H7.
+      apply program_control.
+      rewrite <- H4. assumption.
+      reflexivity.
+      simpl. unfold PLTT.maps_match_on.
+      intros. split; intro; assumption.
+
+  - right.
+    intros E' HE'WF G' HG'WF.
+    eexists. split.
+    (* step *)
+    + destruct (PLTT.split_wellformed G' HG'WF C1 Hcontrol)
+        as [C1I [C1_in_Is C1I_name]].
+      destruct (HmemWF C1I C1 C1_in_Is C1I_name)
+        as [C1mem HC1mem].
+      eapply PLTT.Program_Epsilon.
+      * apply HC1mem.
+      * apply HC1mem.
+      * simpl. unfold PLTT.maps_match_on.
+        intros. split; intro; apply HE'WF; assumption.
+      * simpl. rewrite H3 in H.
+        inversion H.
+        rewrite H4 in Hstep.
+        rewrite H5 in Hstep.
+        rewrite H6 in Hstep.
+        rewrite H7 in Hstep.
+        rewrite H8 in Hstep.
+        eapply Hstep.
+      * apply Hmem. assumption.
+        rewrite H3 in H.
+        inversion H.
+        rewrite <- H4. assumption.
+      * eassumption.
+    (* states match *)
+    + simpl. rewrite H3 in H.
+      inversion H.
+      rewrite <- H7.
+      apply program_control.
+      rewrite <- H4. assumption.
+      reflexivity.
+      simpl. unfold PLTT.maps_match_on.
+      intros. split; intro; assumption.
+
+  (* program is calling *)
+  - right.
+    intros E' HE'WF G' HG'WF.
+    destruct (in_dec Nat.eq_dec C' split) as [ HC'origin | ? ].
+    (* internal call *)
+    + eexists. split.
+      (* step *)
+      * apply PLTT.Program_Internal_Call;
+          try assumption;
+          reflexivity.
+      (* states match *)
+      * unfold PLTT.maps_match_on in HE'WF.
+        destruct
+          (PLTT.split_wellformed G' HG'WF C' HC'origin)
+          as [CI HCI].
+        destruct HCI as [CI_in_Is CI_name_is_C'].
+        destruct (PLTT.entrypoints_exist
+                    G' HG'WF CI C' CI_in_Is CI_name_is_C')
+          as [C'_in_E' [addrs C'_mapsto_E']].
+        rewrite EntryPoint.get_works_locally with
+          (E':=E') (addrs:=addrs).
+        apply program_control;
+          try assumption.
+        ** simpl.
+           apply Util.in_implies_mem_true in Hcontrol.
+           rewrite Hcontrol.
+           reflexivity.
+        ** apply HE'WF. assumption. assumption.
+        ** assumption.
+    (* external call *)
+    + eexists. split.
+      (* step *)
+      * apply PLTT.Program_External_Call;
+          try assumption;
+          reflexivity.
+      (* states match *)
+      * apply context_control.
+        ** assumption.
+        ** simpl.
+           apply Util.in_implies_mem_true in Hcontrol.
+           rewrite Hcontrol.
+           reflexivity.
+        ** assumption.
+
+  (* program is returning *)
+  - right.
+    intros E' HE'WF G' HG'WF.
+    destruct (in_dec Nat.eq_dec C' split)
+      as [ HC'origin | HC'origin ].
+    (* internal return *)
+    + eexists. split.
+      (* step *)
+      * apply PLTT.Program_Internal_Return;
+          try assumption.
+        ** simpl.
+           apply Util.in_implies_mem_true in HC'origin.
+           rewrite HC'origin. reflexivity.
+      (* states match *)
+      * apply program_control;
+          try assumption;
+          reflexivity.
+    (* external return *)
+    + eexists. split.
+      (* step *)
+      * apply PLTT.Program_External_Return;
+          try assumption.
+          ** simpl.
+             apply Util.not_in_implies_mem_false in HC'origin.
+             rewrite HC'origin. reflexivity.
+      (* states match *)
+      * apply context_control;
+          try assumption;
+          reflexivity.
+
+  (* context store *)
+  - unfold PLTT.maps_match_on.
+    intros C' C'mem HC'origin.
+    split.
+    + intro HC'map.
+      apply Hmem.
+      * assumption.
+      * destruct (M.find (elt:=list nat) C1 mem1) eqn:HC1find.
+        ** unfold Memory.set in HC'map.
+           rewrite HC1find in HC'map.
+           apply M.add_3 in HC'map.
+           *** assumption.
+           *** unfold not. intros HeqC1C'.
+               apply Hcontrol.
+               rewrite <- HeqC1C' in HC'origin.
+               apply HC'origin.
+        ** unfold Memory.set in HC'map.
+           rewrite HC1find in HC'map.
+           assumption.
+    + intro HC'map.
+      assert (HneqC1C': C1 <> C').
+      { intro HeqCC'. apply Hcontrol.
+        rewrite <- HeqCC' in HC'origin. apply HC'origin. }
+      unfold Memory.set.
+      * destruct (M.find (elt:=list nat) C1 mem1) eqn:HC1find.
+        ** assert (HC'mem: PLTT.M.MapsTo C' C'mem mem1).
+           { apply Hmem; assumption. }
+           eapply M.add_2; assumption.
+        ** apply Hmem; assumption.
+
+  (* context call is calling *) 
+  - right.
+    destruct (in_dec Nat.eq_dec C' split)
+      as [ HC'origin | ? ];
+      intros E' HE'WF G' HG'WF; eexists; split.
+    (* external call - step *)
+    + apply PLTT.Context_External_Call;
+        try assumption.
+      * apply PLTT.push_by_context_preserves_partial_stack.
+        eassumption.
+        reflexivity.
+    (* external call - states match *)
+    + unfold PLTT.maps_match_on in HE'WF.
+      destruct (PLTT.split_wellformed G' HG'WF C' HC'origin)
+        as [CI HCI].
+      destruct HCI as [CI_in_Is CI_name_is_C'].
+      destruct (PLTT.entrypoints_exist
+                  G' HG'WF CI C' CI_in_Is CI_name_is_C')
+        as [C'_in_E' [addrs C'_mapsto_E']].
+      rewrite EntryPoint.get_works_locally with
+        (E':=E') (addrs:=addrs).
+      apply program_control;
+        try assumption;
+        try reflexivity.
+      * apply (HE'WF C' addrs);
+          assumption.
+      * assumption.
+
+    (* internal call - step *)
+    + apply PLTT.Context_Internal_Call;
+        try assumption.
+      * apply PLTT.push_by_context_preserves_partial_stack.
+        eassumption.
+        reflexivity.
+    (* internal call - states match *)
+    + apply context_control;
+        try assumption;
+        reflexivity.
+
+  (* context is returning *)
+  - right.
+    destruct (in_dec Nat.eq_dec C' split) as [HC'origin | ?];
+      intros E' HE'WF G' HG'WF; eexists; split.
+    (* external return - step*)
+    + apply PLTT.Context_External_Return.
+      * simpl. apply Util.in_implies_mem_true in HC'origin.
+        rewrite HC'origin.
+        reflexivity.
+      * assumption.
+    (* external return - states match *)
+    + apply program_control;
+        try assumption;
+        reflexivity.
+
+    (* internal return - step *)
+    + apply PLTT.Context_Internal_Return.
+      * intro HCeqC'. apply H3. symmetry. apply HCeqC'.
+      * assumption.
+      * apply PLTT.push_by_context_preserves_partial_stack.
+        ** assumption.
+        ** reflexivity.
+    (* internal return - states match *)
+    + apply context_control;
+        try assumption;
+        reflexivity.
+Qed.
+
+End LTT_TO_PLTT.
